processor: solved the Qed-taking-forever issue, added one more Kami-step inversion lemma (needs more refactoring though)

processor/src/KamiProc.v
@@ -3,17 +3,178 @@ Require Import Coq.ZArith.ZArith.
 Require Import Coq.Lists.List. Import ListNotations.
 
 Require Import Kami.
-Require Import Kami.Ex.SC Kami.Ex.IsaRv32 Kami.Ex.SCMMInl.
+Require Import Kami.Ex.MemTypes Kami.Ex.SC Kami.Ex.IsaRv32 Kami.Ex.SCMMInl.
 Require Import Kami.Ex.ProcMemCorrect.
 
 Local Open Scope Z_scope.
+
+Set Implicit Arguments.
+
+Section Parametrized.
+  Variables addrSize iaddrSize fifoSize instBytes dataBytes rfIdx: nat.
+
+  (* External abstract ISA: decoding and execution *)
+  Variables (getOptype: OptypeT instBytes)
+            (getLdDst: LdDstT instBytes rfIdx)
+            (getLdAddr: LdAddrT addrSize instBytes)
+            (getLdSrc: LdSrcT instBytes rfIdx)
+            (calcLdAddr: LdAddrCalcT addrSize dataBytes)
+            (getStAddr: StAddrT addrSize instBytes)
+            (getStSrc: StSrcT instBytes rfIdx)
+            (calcStAddr: StAddrCalcT addrSize dataBytes)
+            (getStVSrc: StVSrcT instBytes rfIdx)
+            (getSrc1: Src1T instBytes rfIdx)
+            (getSrc2: Src2T instBytes rfIdx)
+            (getDst: DstT instBytes rfIdx)
+            (exec: ExecT iaddrSize instBytes dataBytes)
+            (getNextPc: NextPcT iaddrSize instBytes dataBytes rfIdx)
+            (alignAddr: AlignAddrT addrSize)
+            (isMMIO: IsMMIOT addrSize).
+
+  Variable (init: ProcInit iaddrSize dataBytes rfIdx).
+
+  Definition pprocInl :=
+    scmmInl getOptype getLdDst getLdAddr getLdSrc calcLdAddr
+            getStAddr getStSrc calcStAddr getStVSrc
+            getSrc1 getSrc2 getDst exec getNextPc alignAddr
+            isMMIO init.
+
+  Definition pproc := projT1 pprocInl.
+
+  (** The auxiliary hardware state; this is for manipulating hardware state
+   * without knowing much about Kami states.
+   *)
+  Record pst :=
+    mk { pc: word (2 + iaddrSize);
+         rf: word rfIdx -> word (dataBytes * BitsPerByte);
+         pgm: word iaddrSize -> word (instBytes * BitsPerByte);
+         mem: word addrSize -> word (dataBytes * BitsPerByte)
+       }.
+
+  Definition pRegsToT (r: Kami.Semantics.RegsT): option pst :=
+    (mlet pinit: Bool <- r |> "pinit" <| None;
+       if pinit
+       then (mlet pcv: (Pc iaddrSize) <- r |> "pc" <| None;
+               mlet rfv: (Vector (Data dataBytes) rfIdx) <- r |> "rf" <| None;
+               mlet pgmv: (Vector (Data instBytes) iaddrSize) <- r |> "pgm" <| None;
+               mlet memv: (Vector (Data dataBytes) addrSize) <- r |> "mem" <| None;
+               (Some {| pc := pcv;
+                        rf := rfv;
+                        pgm := pgmv;
+                        mem := memv |}))
+       else None)%mapping.
+
+  (** * Inverting Kami rules for instruction executions *)
+
+  Local Definition iaddrSizeZ: Z := Z.of_nat iaddrSize.
+
+  Lemma invert_Kami_execLd_by_memory:
+    forall km1 kt1 kupd klbl,
+      pRegsToT km1 = Some kt1 ->
+      Step pproc km1 kupd klbl ->
+      klbl.(annot) = Some (Some "execLd"%string) ->
+      let curInst := (pgm kt1) (split2 _ _ (pc kt1)) in
+      let ldAddr :=
+          evalExpr
+            (alignAddr
+               _ (evalExpr
+                    (calcLdAddr
+                       _ (evalExpr (getLdAddr _ curInst))
+                       (rf kt1 (evalExpr (getLdSrc _ curInst)))))) in
+      evalExpr (isMMIO _ ldAddr) = false ->
+      exists kt2,
+        klbl.(calls) = FMap.M.empty _ /\
+        pRegsToT (FMap.M.union kupd km1) = Some kt2 /\
+        kt2 = {| pc := evalExpr (getNextPc _ (rf kt1) (pc kt1) curInst);
+                 rf :=
+                   fun w =>
+                     if weq w (evalExpr (getLdDst _ curInst))
+                     then mem kt1 ldAddr
+                     else rf kt1 w;
+                 pgm := pgm kt1;
+                 mem := mem kt1 |}.
+  Proof.
+    intros.
+    kinvert; try (repeat
+                    match goal with
+                    | [H: annot ?klbl = Some _ |- _] => rewrite H in *
+                    | [H: (_ :: _)%struct = (_ :: _)%struct |- _] =>
+                      inversion H; subst; clear H
+                    end; discriminate).
+    kinv_action_dest.
+
+    - unfold pRegsToT in *.
+      kregmap_red.
+      destruct (FMap.M.find "mem"%string km1)
+        as [[[kind|] memv]|]; try discriminate.
+      destruct (decKind kind _); try discriminate.
+      kregmap_red.
+      inversion H; subst; clear H.
+      subst curInst ldAddr.
+      simpl in *.
+      clear -H2 Heqic.
+      congruence.
+    - kinv_red.
+      unfold pRegsToT in *.
+      kregmap_red.
+      inversion H; subst; clear H; simpl in *.
+      eexists; split; [|split].
+      + assumption.
+      + reflexivity.
+      + reflexivity.
+  Qed.
+
+  Lemma invert_Kami_execNm:
+    forall km1 kt1 kupd klbl,
+      pRegsToT km1 = Some kt1 ->
+      Step pproc km1 kupd klbl ->
+      klbl.(annot) = Some (Some "execNm"%string) ->
+      exists kt2,
+        klbl.(calls) = FMap.M.empty _ /\
+        pRegsToT (FMap.M.union kupd km1) = Some kt2 /\
+        exists curInst execVal,
+          curInst = (pgm kt1) (split2 _ _ (pc kt1)) /\
+          execVal = evalExpr
+                      (exec
+                         _
+                         (rf kt1 (evalExpr (getSrc1 _ curInst)))
+                         (rf kt1 (evalExpr (getSrc2 _ curInst)))
+                         (pc kt1)
+                         curInst) /\
+          kt2 = {| pc := evalExpr (getNextPc _ (rf kt1) (pc kt1) curInst);
+                   rf :=
+                     fun w =>
+                       if weq w (evalExpr (getDst type curInst))
+                       then execVal else rf kt1 w;
+                   pgm := pgm kt1;
+                   mem := mem kt1 |}.
+  Proof.
+    intros.
+    kinvert; try (repeat
+                    match goal with
+                    | [H: annot ?klbl = Some _ |- _] => rewrite H in *
+                    | [H: (_ :: _)%struct = (_ :: _)%struct |- _] =>
+                      inversion H; subst; clear H
+                    end; discriminate).
+    kinv_action_dest.
+    unfold pRegsToT in *.
+    kregmap_red.
+    destruct (FMap.M.find "mem"%string km1)
+      as [[[kind|] memv]|]; try discriminate.
+    destruct (decKind kind _); try discriminate.
+    kregmap_red.
+    inversion H; subst; clear H.
+    repeat esplit.
+    assumption.
+  Qed.
+  
+End Parametrized.
 
 Definition width: Z := 32.
 Definition width_cases: width = 32 \/ width = 64 := or_introl eq_refl.
 Local Notation nwidth := (Z.to_nat width).
 
-Definition isMMIO: IsMMIOT nwidth :=
-  (fun _ addr => ($$false)%kami_expr).
+Definition isMMIO: IsMMIOT nwidth := cheat _.
 
 Section PerInstAddr.
   Context {instrMemSizeLg: Z}.
@@ -26,40 +187,24 @@ Section PerInstAddr.
   Definition predictNextPc ty (ppc: fullType ty (SyntaxKind (Pc ninstrMemSizeLg))) :=
     (#ppc + $4)%kami_expr.
 
-  Definition scmmInl :=
-    @scmmInl
-      nwidth ninstrMemSizeLg
-      rv32InstBytes rv32DataBytes rv32RfIdx rv32GetOptype
-      rv32GetLdDst (rv32GetLdAddr _) rv32GetLdSrc (rv32CalcLdAddr _)
+  Definition procInl :=
+    pprocInl
+      rv32GetOptype rv32GetLdDst (rv32GetLdAddr _) rv32GetLdSrc (rv32CalcLdAddr _)
       (rv32GetStAddr _) rv32GetStSrc (rv32CalcStAddr _) rv32GetStVSrc
       rv32GetSrc1 rv32GetSrc2 rv32GetDst (rv32Exec _)
       (rv32NextPc _) (rv32AlignAddr _)
       isMMIO procInit.
 
-  Definition proc: Kami.Syntax.Modules := projT1 scmmInl.
+  Definition proc: Kami.Syntax.Modules := projT1 procInl.
 
   Definition hst := Kami.Semantics.RegsT.
 
   (** Abstract hardware state *)
-  Record st :=
-    mk { pc: word (2 + ninstrMemSizeLg);
-         rf: word rv32RfIdx -> word nwidth;
-         pgm: word ninstrMemSizeLg -> word nwidth;
-         mem: word nwidth -> word nwidth
-       }.
+  Definition st :=
+    @pst nwidth ninstrMemSizeLg rv32InstBytes rv32DataBytes rv32RfIdx.
 
   Definition RegsToT (r: hst): option st :=
-    (mlet pinit: Bool <- r |> "pinit" <| None;
-       if pinit
-       then (mlet pcv: (Pc ninstrMemSizeLg) <- r |> "pc" <| None;
-               mlet rfv: (Vector (Bit nwidth) rv32RfIdx) <- r |> "rf" <| None;
-               mlet pgmv: (Vector (Bit nwidth) ninstrMemSizeLg) <- r |> "pgm" <| None;
-               mlet memv: (Vector (Bit nwidth) nwidth) <- r |> "mem" <| None;
-               (Some {| pc := pcv;
-                        rf := rfv;
-                        pgm := pgmv;
-                        mem := memv |}))
-       else None)%mapping.
+    pRegsToT nwidth ninstrMemSizeLg rv32InstBytes rv32DataBytes rv32RfIdx r.
 
   (** Refinement from [p4mm] to [proc] (as a spec) *)
 
@@ -75,7 +220,7 @@ Section PerInstAddr.
   Proof.
     ketrans.
     - apply p4mm_correct. (* [p4mm] refines [scmm] *)
-    - apply (projT2 scmmInl). (* [scmm] refines [projT1 scmmInl], the inlined module. *)
+    - apply (projT2 procInl). (* [scmm] refines [projT1 scmmInl], the inlined module. *)
   Qed.
 
 End PerInstAddr.
